src/SDK/Serialize/SerializeFunctions.dfy
@@ -27,23 +27,24 @@ module SerializeFunctions {
     | Error(message: string)
   type MoreNeeded = p: ReadProblems | p.MoreNeeded? witness *
 
-
-  datatype ReadableBytes = ReadableBytes(
-    data: seq<uint8>,
+  // When reading a buffer,
+  // there are the bytes to read,
+  // and the position to start reading withing these bytes.
+  // This data structure represents this information.
+  datatype ReadableBuffer = ReadableBuffer(
+    bytes: seq<uint8>,
     start: nat
   )
-  datatype Data<T> = Data(
-    thing: T,
-    tail: ReadableBytes
+
+  // This holds the data from a successful read.
+  // The `data` is the read type,
+  // and the `tail` is the remaining data left to be read.
+  datatype SuccessfulRead<T> = SuccessfulRead(
+    data: T,
+    tail: ReadableBuffer
   )
 
-  // Think about a type
-  // datatype Thing = Thing(data: s:seq<uint8>, pos: nat)
-  // Then we take and return this thing,
-  // not just `pos`.
-  // Currently we use a tuple,
-  // but a more complete datatype like above may be better long term.
-  type ReadResult<T, E> = Result<Data<T>, E>
+  type ReadResult<T, E> = Result<SuccessfulRead<T>, E>
   type ReadCorrect<T> = ReadResult<T, ReadProblems>
   // When reading binary it can not be incorrect.
   // It may not be enough data, but since it is raw binary,
@@ -53,27 +54,40 @@ module SerializeFunctions {
   // it may be other types.
   type ReadBinaryCorrect<T> = ReadResult<T, MoreNeeded>
 
-  predicate CorrectlyReadRange(
-    bytes: ReadableBytes,
-    tail: ReadableBytes
-  )
-  {
-    && tail.data == bytes.data
-    && bytes.start <= tail.start <= |tail.data|
-    && bytes.data[bytes.start..tail.start] == tail.data[bytes.start..tail.start]
-  }
-
+  // This is the composable unit
+  // that all `ReadX` functions use to prove correctness. 
+  // The idea is that WriteX(ReadX(ReadableBuffer)) == ReadableBuffer.
+  // That a read is the inverse of a write.
+  // This puts the correctness on the write side,
+  // and the read side is correct _because_
+  // what was read is what would have been written.
   predicate CorrectlyRead<T> (
-    bytes: ReadableBytes,
+    buffer: ReadableBuffer,
     res: ReadCorrect<T>,
     invertT: T -> seq<uint8>
   )
   {
     res.Success?
     ==>
-      && var Data(thing, tail) := res.value;
-      && CorrectlyReadRange(bytes, tail)
-      && invertT(thing) == tail.data[bytes.start..tail.start]
+      && var SuccessfulRead(thing, tail) := res.value;
+      && CorrectlyReadRange(buffer, tail)
+      && invertT(thing) == tail.bytes[buffer.start..tail.start]
+  }
+
+  // Sequence ranges are complicated in Dafny.
+  // By separating out the sub sequence
+  // (the bytes under consideration)
+  // it is easer to prove associativity.
+  // See: ConsecutiveReadsAreAssociative
+  // e.g. bytes[start..stop] == bytes[start..mid] + bytes[mid..stop];
+  predicate CorrectlyReadRange(
+    buffer: ReadableBuffer,
+    tail: ReadableBuffer
+  )
+  {
+    && tail.bytes == buffer.bytes
+    && buffer.start <= tail.start <= |tail.bytes|
+    && buffer.bytes[buffer.start..tail.start] == tail.bytes[buffer.start..tail.start]
   }
 
   // This function is trivial,
@@ -91,7 +105,7 @@ module SerializeFunctions {
   }
 
   function method {:opaque} Read(
-    bytes: ReadableBytes,
+    buffer: ReadableBuffer,
     length: nat
   ):
     (res: ReadBinaryCorrect<seq<uint8>>)
@@ -99,29 +113,29 @@ module SerializeFunctions {
     // however given compositional it is much more common than you might think.
     // Optional elements in a data structure can be represented with a length of 0 bytes.
     ensures
-      && |bytes.data| >= bytes.start + length
+      && |buffer.bytes| >= buffer.start + length
     ==>
       && res.Success?
     ensures
-      && |bytes.data| < bytes.start + length
+      && |buffer.bytes| < buffer.start + length
     ==>
       && res.Failure?
       && res.error.MoreNeeded?
-      && res.error.pos == bytes.start + length
-    ensures CorrectlyRead(bytes, res, Write)
+      && res.error.pos == buffer.start + length
+    ensures CorrectlyRead(buffer, res, Write)
     ensures res.Success?
     ==>
-      var Data(thing, tail) := res.value;
+      var SuccessfulRead(thing, tail) := res.value;
       && |thing| == length
-      && tail.start == bytes.start + length
-      && tail.data[bytes.start..tail.start] == thing
+      && tail.start == buffer.start + length
+      && tail.bytes[buffer.start..tail.start] == thing
   {
-    var end := bytes.start + length;
-    :- Need(|bytes.data| >= end, MoreNeeded(end));
+    var end := buffer.start + length;
+    :- Need(|buffer.bytes| >= end, MoreNeeded(end));
 
-    Success(Data(
-      bytes.data[bytes.start..end],
-      bytes.(start := end)))
+    Success(SuccessfulRead(
+      buffer.bytes[buffer.start..end],
+      buffer.(start := end)))
   }
 
   function method WriteUint16(
@@ -134,13 +148,13 @@ module SerializeFunctions {
 
   // Opaque? Because the body is not interesting...
   function method ReadUInt16(
-    bytes: ReadableBytes
+    buffer: ReadableBuffer
   )
     :(res: ReadBinaryCorrect<uint16>)
-    ensures CorrectlyRead(bytes, res, WriteUint16)
+    ensures CorrectlyRead(buffer, res, WriteUint16)
   {
-    var Data(uint16Bytes, tail) :- Read(bytes, 2);
-    Success(Data(SeqToUInt16(uint16Bytes), tail))
+    var SuccessfulRead(uint16Bytes, tail) :- Read(buffer, 2);
+    Success(SuccessfulRead(SeqToUInt16(uint16Bytes), tail))
   }
 
   function method WriteUint32(
@@ -152,13 +166,13 @@ module SerializeFunctions {
   }
 
   function method ReadUInt32(
-    bytes: ReadableBytes
+    buffer: ReadableBuffer
   ):
     (res: ReadBinaryCorrect<uint32>)
-    ensures CorrectlyRead(bytes, res, WriteUint32)
+    ensures CorrectlyRead(buffer, res, WriteUint32)
   {
-    var Data(uint32Bytes, tail) :- Read(bytes, 4);
-    Success(Data(SeqToUInt32(uint32Bytes), tail))
+    var SuccessfulRead(uint32Bytes, tail) :- Read(buffer, 4);
+    Success(SuccessfulRead(SeqToUInt32(uint32Bytes), tail))
   }
 
   function method WriteUint64(
@@ -170,13 +184,13 @@ module SerializeFunctions {
   }
 
   function method ReadUInt64(
-    bytes: ReadableBytes
+    buffer: ReadableBuffer
   ):
     (res: ReadBinaryCorrect<uint64>)
-    ensures CorrectlyRead(bytes, res, UInt64ToSeq)
+    ensures CorrectlyRead(buffer, res, UInt64ToSeq)
   {
-    var Data(uint64Bytes, tail) :- Read(bytes, 8);
-    Success(Data(SeqToUInt64(uint64Bytes), tail))
+    var SuccessfulRead(uint64Bytes, tail) :- Read(buffer, 8);
+    Success(SuccessfulRead(SeqToUInt64(uint64Bytes), tail))
   }
 
   function method WriteShortLengthSeq(
@@ -189,13 +203,13 @@ module SerializeFunctions {
   }
 
   function method ReadShortLengthSeq(
-    bytes: ReadableBytes
+    buffer: ReadableBuffer
   ):
     (res: ReadCorrect<Uint8Seq16>)
-    ensures CorrectlyRead(bytes, res, WriteShortLengthSeq)
+    ensures CorrectlyRead(buffer, res, WriteShortLengthSeq)
   {
-    var length :- ReadUInt16(bytes);
-    var d: Data<Uint8Seq16> :- Read(length.tail, length.thing as nat);
+    var length :- ReadUInt16(buffer);
+    var d: SuccessfulRead<Uint8Seq16> :- Read(length.tail, length.data as nat);
     Success(d)
   }
 
@@ -209,13 +223,13 @@ module SerializeFunctions {
   }
 
   function method ReadUint32Seq(
-    bytes: ReadableBytes
+    buffer: ReadableBuffer
   ):
     (res: ReadCorrect<Uint8Seq32>)
-    ensures CorrectlyRead(bytes, res, WriteUint32Seq)
+    ensures CorrectlyRead(buffer, res, WriteUint32Seq)
   {
-    var length :- ReadUInt32(bytes);
-    var d: Data<Uint8Seq32> :- Read(length.tail, length.thing as nat);
+    var length :- ReadUInt32(buffer);
+    var d: SuccessfulRead<Uint8Seq32> :- Read(length.tail, length.data as nat);
     Success(d)
   }
 
@@ -229,34 +243,34 @@ module SerializeFunctions {
   }
 
   function method ReadUint64Seq(
-    bytes: ReadableBytes
+    buffer: ReadableBuffer
   ):
     (res: ReadCorrect<Uint8Seq64>)
-    ensures CorrectlyRead(bytes, res, WriteUint64Seq)
+    ensures CorrectlyRead(buffer, res, WriteUint64Seq)
   {
-    var length :- ReadUInt64(bytes);
-    var d: Data<Uint8Seq64> :- Read(length.tail, length.thing as nat);
+    var length :- ReadUInt64(buffer);
+    var d: SuccessfulRead<Uint8Seq64> :- Read(length.tail, length.data as nat);
     Success(d)
   }
 
   // Combining consecutive reads can be problematic for Dafny to prove `CorrectlyRead`.
-  // This lemma aims to simplify this by proving
-  // that the total bytes read is equal to the sum of all `Read` calls.
+  // This lemma aims to simplify this
+  // by proving that the total bytes read is equal to the sum of all `Read` calls.
   // This lemma works for any function
   // that uses `Read`, `CorrectlyRead` and `CorrectlyReadRange`
   // as the basis for its correctness.
   // A simple example is to prove the following assert:
   // 
-  //  var first :- Read(bytes, a);
-  //  var second :- Read(bytes, b);
-  //  var third :- Read(bytes, c);
-  //  var fourth :- Read(bytes, d);
-  //  assert fourth.tail.data[bytes.start..fourth.tail]
-  //  == fourth.tail.data[bytes.start..first.tail.start]
+  //  var first :- Read(buffer, a);
+  //  var second :- Read(buffer, b);
+  //  var third :- Read(buffer, c);
+  //  var fourth :- Read(buffer, d);
+  //  assert fourth.tail.data[buffer.start..fourth.tail]
+  //  == fourth.tail.data[buffer.start..first.tail.start]
   //  + fourth.tail.data[first.tail.start..second.tail.start]
   //  + fourth.tail.data[second.tail.start..third.tail.start]
   //  + fourth.tail.data[third.tail.start..fourth.tail.start]
-  lemma ConsecutiveReadsAreAssociative(positions: seq<ReadableBytes>)
+  lemma ConsecutiveReadsAreAssociative(positions: seq<ReadableBuffer>)
     requires |positions| >= 2
     requires PositionsAreConsecutive(positions)
 
@@ -284,13 +298,13 @@ module SerializeFunctions {
   }
 
   // This ensures that all the `start` positions
-  // in the seq of ReadableBytes
+  // in the seq of ReadableBuffer
   // are moving "down" the binary data.
   // The goal is that these positions
   // come from a sequence of consecutive `Read`
   // or more complicated `Read*` calls.
   predicate PositionsAreConsecutive(
-    positions: seq<ReadableBytes>
+    positions: seq<ReadableBuffer>
   )
   {
     forall i,j
@@ -303,8 +317,8 @@ module SerializeFunctions {
   // and therefore represents a range.
   // e.g. the start of the last read to the start of the next read.
   // This function translates these positions into these ranges.
-  function PositionsToReadableRanges(positions: seq<ReadableBytes>)
-    :(ranges: seq<(ReadableBytes, ReadableBytes)>)
+  function PositionsToReadableRanges(positions: seq<ReadableBuffer>)
+    :(ranges: seq<(ReadableBuffer, ReadableBuffer)>)
     requires |positions| >= 2
     requires PositionsAreConsecutive(positions)
 
@@ -330,7 +344,7 @@ module SerializeFunctions {
   // in a way that makes it easy to prove
   // that it is equal to the "complete range"
   // e.g. the very first read position, to the very last read position.
-  function ConcatenateRanges(ranges: seq<(ReadableBytes, ReadableBytes)>)
+  function ConcatenateRanges(ranges: seq<(ReadableBuffer, ReadableBuffer)>)
     :(ret: seq<uint8>)
     requires forall i,j
     | 0 <= i < j < |ranges| && i + 1 == j
@@ -352,12 +366,12 @@ module SerializeFunctions {
   // Given a range, please read it.
   // Just sugar to make things more readable.
   function ReadRange(
-    range: (ReadableBytes, ReadableBytes)
+    range: (ReadableBuffer, ReadableBuffer)
   )
     :(ret: seq<uint8>)
     requires CorrectlyReadRange(range.0, range.1)
   {
-    range.1.data[range.0.start..range.1.start]
+    range.1.bytes[range.0.start..range.1.start]
   }
 
 }
